src/Distributions/Uniform/Model.dfy
@@ -19,7 +19,7 @@ module Uniform.Model {
   opaque ghost function {:axiom} Sample(n: nat): (h: Monad.Hurd<nat>)
     requires n > 0
     ensures Independence.IsIndep(h)
-    ensures forall s :: h(s).Result? ==> 0 <= h(s).value < n
+    ensures forall s :: 0 <= h(s).value < n
 
   ghost function IntervalSample(a: int, b: int): (f: Monad.Hurd<int>)
     requires a < b
@@ -33,13 +33,11 @@ module Uniform.Model {
 
   lemma SampleBound(n: nat, s: Rand.Bitstream)
     requires n > 0
-    requires Sample(n)(s).Result?
     ensures 0 <= Sample(n)(s).value < n
   {}
 
   lemma IntervalSampleBound(a: int, b: int, s: Rand.Bitstream)
     requires a < b
-    requires IntervalSample(a, b)(s).Result?
     ensures a <= IntervalSample(a, b)(s).value < b
   {
     SampleBound(b-a, s);
