src/Util/FisherYates/Implementation.dfy
@@ -20,6 +20,7 @@ module FisherYates.Implementation {
       ghost var prevI, prevASeq, prevS := 0, a[..], s; // ghost
       if a.Length > 1 {
         for i := 0 to a.Length - 1
+          invariant i < a.Length
           invariant Equivalence.LoopInvariant(prevI, i, a, prevASeq, old(a[..]), old(s), prevS, s)
         {
           prevI, prevASeq, prevS := i, a[..], s; // ghost
